Nearly completed DeltaCorrectness. One more proof to clean (currently has an admit, but has been proven before).

Security/SaberRqDeltaCorrectness.ec
@@ -23,6 +23,67 @@ require import SaberRqPreliminaries.
 (*  General Properties                 *)
 (* ----------------------------------- *)
 
+(* --- Convenient Equalities --- *)
+lemma eq_q2_2eq1 : q %/ 2 = 2 ^ (eq - 1).
+proof.
+by rewrite /q (_ :  2 ^ eq =  2 ^ (eq - 1) * 2) 2:mulzK 1:-{3}expr1 1:-exprD_nneg //; smt(ge3_eq).
+qed.
+
+lemma eq_q4_2eq2 : q %/ 4 = 2 ^ (eq - 2).
+proof.
+rewrite /q (_ :  2 ^ eq =  2 ^ (eq - 2) * 4) 2:mulzK //. 
+by rewrite (_ : 4 = 2 ^ 2) 1:expr2 //-exprD_nneg; smt(ge3_eq).
+qed.
+
+lemma eq_q4t_2eqet2 : q %/ (4 * t) = 2 ^ (eq - et - 2).
+proof.
+rewrite /q /t (_ :  2 ^ eq =  2 ^ (eq - et - 2) * (4 * 2 ^ et)) 2:mulzK //.
++ rewrite 1:(_ : 4 = 2 ^ 2) 1:expr2 // -exprD_nneg 2:ge0_et // -exprD_nneg;
+          1, 2:smt(ge0_et geet2_ep geep1_eq).
+  by congr; ring.
++ by rewrite neq_ltz; right; rewrite mulr_gt0 2:expr_gt0.
+qed.
+
+lemma eq_q_14q_34q : q = q %/ 4 + 3 * (q %/ 4).
+proof.
+rewrite eq_q4_2eq2 -{1}(Ring.IntID.mulr1z (2 ^ (eq - 2))) intmulz mulzC -mulrDl /=. 
+by rewrite (_  : 4 = 2 ^ 2) 1:expr2 // -exprD_nneg //; smt(ge3_eq).
+qed.
+
+lemma eq_q2_q4q4 : q %/ 2 = q %/ 4 + q %/ 4.
+proof.
+rewrite eq_q2_2eq1 eq_q4_2eq2 (_ : 2 ^ (eq - 1) = 2 * 2 ^ (eq - 2)).
++ rewrite -{2}expr1 -exprD_nneg; smt(ge3_eq).
+by rewrite mulrC -intmulz mulr2z.
+qed.
+
+lemma eq_upscaleRqh2_q4minq4t : upscaleRq h2 (eq - ep) = q4_Rq - q4t_Rq.
+proof.
+rewrite /upscaleRq polyXnD1_sumN -(BigRq.XnD1CA.big_split) /=.
+rewrite !(BigRq.XnD1CA.big_seq) &(BigRq.XnD1CA.eq_bigr) /= => i /mem_range rng_i.
+rewrite -scaleN -scaleDl; congr.
+rewrite /h2 rcoeffZ_sum //= /upscaleZq /upscale /shl -inzmodD !inzmodK -eq_inzmod /=.
+rewrite modzMml (pmod_small (2 ^ (eq - et - 2))).
++ by rewrite /q expr_ge0 //= ltz_weexpn2l //; smt(geet2_ep geep1_eq ge3_eq ge0_et).
+rewrite mulrBl -!exprD_nneg; first 4 smt(ge2_ep geet2_ep geep1_eq ge3_eq ge0_et).
+have ->: ep - 2 + (eq - ep) = eq - 2 by ring.
+by have ->: ep - et - 2 + (eq - ep) = eq - et - 2 by ring.
+qed.
+
+lemma eq_minq4_q34_modq : Zq.inzmod (- q %/ 4) = Zq.inzmod (3 * (q %/ 4)).
+proof.
+rewrite -eq_inzmod /q {1 3}(_ : 2 ^ eq = 2 ^ (eq - 2) * 4) 1:(_ : 4 = 2 ^ 2) 1:expr2 // 1:-exprD_nneg;
+        1, 2, 3: smt(ge3_eq).
+rewrite !mulzK // modNz 1,2:expr_gt0 // !pmod_small.
++ by rewrite -(lez_add2r 1) /= exprn_ege1 //= 2:-(ltz_add2r 1) /= 2:-(Ring.IntID.addr0 (2 ^ (eq - 2)))
+            2:ltr_add 2:ltz_weexpn2l //=; smt(ge3_eq).
++ by rewrite mulr_ge0 2:expr_ge0 //= (_ : 2 ^ eq = 4 * 2 ^ (eq - 2)) 1:(_ : 4 = 2 ^ 2)
+            1:expr2 // 1:-exprD_nneg 4:ltr_pmul2r 4:expr_gt0 //; smt(ge3_eq).
+rewrite opprD /= addrA; ring; rewrite mulNr (_ : 4 = 2 ^ 2) 1:expr2 // -exprD_nneg; 1, 2: smt(ge3_eq).
+by rewrite addzA (addzC _ (-2)) addzA.
+qed.
+
+(* --- Relevant Matrix/Vector Properties --- *)
 lemma dotpDl_N (pv1 pv2 pv3 : Rq_vec) :
   - dotp (pv1 + pv2) pv3 = - dotp pv1 pv3 - dotp pv2 pv3.
 proof. by rewrite dotpDl opprD. qed.
@@ -39,43 +100,114 @@ lemma dotpRed_Asserr (_A : Rq_mat) (s s': Rq_vec) (err err': Rq_vec) :
 proof. by rewrite dotpDlxTvxv addrC dotpDl opprD; ring. qed.
 *)
 
-lemma eqv_q2_2eq1 : q %/ 2 = 2 ^ (eq - 1).
+(* --- Relevant Scaling Properties --- *)
+lemma scaleZ22Zq2Z2t2Zq_inv (z : Z2) : scaleZ2t2Zq (scaleZq2Z2t (scaleZ22Zq z)) = scaleZ22Zq z.
 proof.
-by rewrite /q (_ :  2 ^ eq =  2 ^ (eq - 1) * 2) 2:mulzK 1:-{3}expr1 1:-exprD_nneg //; smt(ge3_eq).
+rewrite /scaleZ2t2Zq /scaleZq2Z2t /upscale /downscale /shl /shr !inzmodK /t -{2}(Ring.IntID.expr1 2)
+        -exprD_nneg 2:ge0_et // (Ring.IntID.addrC 1 et) -eq_inzmod.
+have: upscale (asint z) eq 1 = 0 \/ upscale (asint z) eq 1 = 2 ^ (eq - 1).
++ by move: (Z2_asint_values z); case => ->.
+case => -> // @/q.
+rewrite modz_pow2_mul; 2: do 2! congr; 2: rewrite -eqz_div 1:neq_ltz 1:expr_gt0 3:dvdz_exp2l //; 
+        first 2 smt(ge0_et geet2_ep geep1_eq). 
+by rewrite pmod_small 1:expr_ge0 2:ltz_weexpn2l; smt(ge3_eq).
 qed.
 
-lemma eqv_q4_2eq2 : q %/ 4 = 2 ^ (eq - 2).
+(* --- Equivalences Regarding Ranges of Coefficients and Results of Scaling --- *)
+(* - Integers - *)
+lemma scaleZq2Z2_rng_zero (z : Zq) : 
+  Zq.asint Zq.zero <= Zq.asint z < Zq.asint (Zq.inzmod (q %/ 2)) <=> scaleZq2Z2 z = Z2.zero.
 proof.
-rewrite /q (_ :  2 ^ eq =  2 ^ (eq - 2) * 4) 2:mulzK //. 
-by rewrite (_ : 4 = 2 ^ 2) 1:expr2 //-exprD_nneg; smt(ge3_eq).
+rewrite eq_q2_2eq1 zeroE inzmodK pmod_small 1:expr_ge0 2:ltz_weexpn2l //; 1, 2, 3: smt(ge3_eq). 
+split => [|eq0_scale].
++ by case => [ge0_z ltq2_z @/scaleZq2Z2 @/downscale @/shr]; rewrite pdiv_small.  
++ split => [|?].
+  - by rewrite Zq.ge0_asint.
+  - move: eq0_scale; rewrite &(contraLR) ltzNge /=; move: (Zq.gtp_asint z) => @/q ltq_z geq2_z.
+    have ->: (scaleZq2Z2 z <> Z2.zero) = (scaleZq2Z2 z = Z2.one).
+    * move: (Z2_asint_values (scaleZq2Z2 z)); rewrite -zeroE -oneE 2!asint_eq.
+      case => -> /=; rewrite -eq_inzmod //.    
+    rewrite /scaleZq2Z2 /downscale /shr -eq_inzmod; do 2! congr.
+    rewrite eqz_leq -(ler_add2l 1) lez_add1r /= ltz_divLR 2:lez_divRL 1,2:expr_gt0 //=.
+    by rewrite -{1}expr1 -exprD_nneg; 2: smt(ge3_eq).
 qed.
 
-lemma eqv_q4t_2eqet2 : q %/ (4 * t) = 2 ^ (eq - et - 2).
+lemma scaleZq2Z2_rng_zero_q4 (z : Zq) :
+  Zq.asint (Zq.inzmod (- q %/ 4)) <= Zq.asint z \/ Zq.asint z < Zq.asint (Zq.inzmod (q %/ 4))
+  <=> 
+  scaleZq2Z2 (Zq.inzmod (q %/ 4) + z) = Z2.zero.
 proof.
-rewrite /q /t (_ :  2 ^ eq =  2 ^ (eq - et - 2) * (4 * 2 ^ et)) 2:mulzK //.
-+ rewrite 1:(_ : 4 = 2 ^ 2) 1:expr2 // -exprD_nneg 2:ge0_et // -exprD_nneg;
-          1, 2:smt(ge0_et geet2_ep geep1_eq).
-  by congr; ring.
-+ by rewrite neq_ltz; right; rewrite mulr_gt0 2:expr_gt0.
+rewrite eq_minq4_q34_modq -scaleZq2Z2_rng_zero zeroE ge0_asint /= !inzmodK 2?pmod_small 
+        3:(pmod_small (q %/ 2)).
++ by rewrite mulr_ge0 2:divz_ge0 3:expr_ge0 //= -(Ring.IntID.add0r (3 * (q %/ 4))) {2}eq_q_14q_34q
+          ltz_add2r eq_q4_2eq2 expr_gt0.
++ by rewrite {1}eq_q4_2eq2 expr_ge0 //= ltz_divLR 2:ltr_pmulr 2:expr_gt0.
++ by rewrite {1}eq_q2_2eq1 expr_ge0 //= ltz_divLR 2:ltr_pmulr 2:expr_gt0.
+split; first case.
++ move: (Zq.gtp_asint z) => ltq_z ge34q_z.
+  pose x := q %/ 4 + asint z - q; have ->: q %/ 4 + asint z = q + x.
+  - by rewrite /x; ring.
+  have [ge0_x ltq2_x]: 0 <= x < q %/ 2; first split => @/x [|?].
+  - by rewrite subr_ge0 {1}eq_q_14q_34q lez_add2l.
+  - rewrite ltr_subl_addl addrC ltr_add // eq_q2_2eq1 eq_q4_2eq2 ltz_weexpn2l //; smt(ge3_eq).
+  by rewrite modzDl !pmod_small 1:(ltr_trans (q %/ 2)) // ltz_divLR 2:ltr_pmulr 2:expr_gt0.
++ move: (Zq.ge0_asint z) => ge0_z ltq4_z.
+  rewrite pmod_small 2:eq_q2_q4q4 2:ltr_add2l // addr_ge0 1:eq_q4_2eq2 1:expr_ge0 //=.
+  by rewrite (ltr_trans (q  %/ 2)) 1:eq_q2_q4q4 1:ltz_add2l // ltz_divLR 2:ltr_pmulr 2:expr_gt0.
++ rewrite &(contraLR) negb_or -!ltzNge /= -!lezNgt /=; move: (Zq.rg_asint z).
+  case => ge0_z ltq_z; case => ltq34_z geq2_z.
+  rewrite eq_q2_q4q4 pmod_small 1:addr_ge0 1:divz_ge0 2:expr_ge0 //= 1:{2}eq_q_14q_34q 1:ltz_add2l //.
+  by rewrite lez_add2l.
 qed.
 
-lemma eq_q_14q_34q : q = q %/ 4 + 3 * (q %/ 4).
+lemma scaleZq2Z2_DM_invl_extract_rng (z1 : Z2) (z2 : Zq) :
+  Zq.asint Zq.zero <= Zq.asint z2 < Zq.asint (Zq.inzmod (q %/ 2)) 
+  <=> 
+  z1 = scaleZq2Z2 (scaleZ22Zq z1 + z2).
 proof.
-rewrite eqv_q4_2eq2 -{1}(Ring.IntID.mulr1z (2 ^ (eq - 2))) intmulz mulzC -mulrDl /=. 
-by rewrite (_  : 4 = 2 ^ 2) 1:expr2 // -exprD_nneg //; smt(ge3_eq).
+rewrite scaleZq2Z2_DM_invl (_ : (z1 = z1 + (scaleZq2Z2 z2)) <=> ((scaleZq2Z2 z2) = Z2.zero)).
++ split => equ.
+  - by rewrite &(Z2.ZModpRing.addrI z1) Z2.ZModpRing.addr0 eq_sym.
+  - by rewrite &(Z2.ZModpRing.addrI (- z1)) Z2.ZModpRing.addrA Z2.ZModpRing.addrC Z2.ZModpRing.subrr
+               Z2.ZModpRing.add0r eq_sym.
++ by apply scaleZq2Z2_rng_zero.
 qed.
 
-lemma eq_minq4_q34_modq : Zq.inzmod (- q %/ 4) = Zq.inzmod (3 * (q %/ 4)).
+(* - Polynomials - *)
+lemma scaleRq2R2_rng_zero (p : Rq) : 
+  (forall (i : int), 0 <= i < n => Zq.asint Zq.zero <= Zq.asint p.[i] < Zq.asint (Zq.inzmod (q %/ 2)))
+  <=> 
+  (scaleRq2R2 p = R2.zeroXnD1).
 proof.
-rewrite -eq_inzmod /q {1 3}(_ : 2 ^ eq = 2 ^ (eq - 2) * 4) 1:(_ : 4 = 2 ^ 2) 1:expr2 // 1:-exprD_nneg;
-        1, 2, 3: smt(ge3_eq).
-rewrite !mulzK // modNz 1,2:expr_gt0 // !pmod_small.
-+ by rewrite -(lez_add2r 1) /= exprn_ege1 //= 2:-(ltz_add2r 1) /= 2:-(Ring.IntID.addr0 (2 ^ (eq - 2)))
-            2:ltr_add 2:ltz_weexpn2l //=; smt(ge3_eq).
-+ by rewrite mulr_ge0 2:expr_ge0 //= (_ : 2 ^ eq = 4 * 2 ^ (eq - 2)) 1:(_ : 4 = 2 ^ 2)
-            1:expr2 // 1:-exprD_nneg 4:ltr_pmul2r 4:expr_gt0 //; smt(ge3_eq).
-rewrite opprD /= addrA; ring; rewrite mulNr (_ : 4 = 2 ^ 2) 1:expr2 // -exprD_nneg; 1, 2: smt(ge3_eq).
-by rewrite addzA (addzC _ (-2)) addzA.
+split => [coeff_rng|]; rewrite polyXnD1_eqP => [i rng_i| coeff_scale i rng_i]; 
+         2: move: (coeff_scale i rng_i); rewrite rcoeffZ_sum //= rcoeff0 -scaleZq2Z2_rng_zero //. 
++ by apply (coeff_rng i rng_i).
+qed.
+
+lemma scaleRq2R2_rng_zero_q4 (p : Rq) :
+  (forall (i : int), 0 <= i < n =>
+   Zq.asint (Zq.inzmod (- q %/ 4)) <= Zq.asint p.[i] 
+   \/ Zq.asint p.[i] < Zq.asint (Zq.inzmod (q %/ 4)))
+  <=> 
+  scaleRq2R2 (q4_Rq + p) = R2.zeroXnD1.
+proof.
+split => [coeff_rng|]; rewrite polyXnD1_eqP => [i rng_i| coeff_scale i rng_i];
+         2: move: (coeff_scale i rng_i); rewrite rcoeffZ_sum //= (Rq.rcoeffD q4_Rq p) rcoeff0
+         rcoeffZ_sum //= -/(Zq.Sub.insubd (2 ^ (eq - 2) %% q)) -/(Zq.inzmod ((2 ^ (eq - 2))))
+         -eq_q4_2eq2 -(scaleZq2Z2_rng_zero_q4 p.[i]) //.
++ by apply (coeff_rng i rng_i).
+qed.
+
+lemma scaleRq2R2_DM_invl_extract_rng (p1 : R2) (p2 : Rq) :
+  (forall (i : int), 0 <= i < n => 
+   Zq.asint Zq.zero <= Zq.asint p2.[i] < Zq.asint (Zq.inzmod (q %/ 2)))
+  <=>
+  p1 = scaleRq2R2 (scaleR22Rq p1 + p2).
+proof.
+split => [coeff_rng|]; rewrite polyXnD1_eqP => [i rng_i| coeff_scale i rng_i];
+         2: move: (coeff_scale i rng_i); rewrite rcoeffZ_sum //= rcoeffD rcoeffZ_sum //=
+         -scaleZq2Z2_DM_invl_extract_rng //.
++ by apply (coeff_rng i rng_i).
 qed.
 
 (* ----------------------------------- *)
@@ -85,6 +217,8 @@ qed.
 module type Adv_Cor = {
    proc choose(pk : pkey, sk : skey) : plaintext
 }.
+
+axiom Adv_Cor_ll (A <: Adv_Cor) : islossless A.choose.
 
 (* ----------------------------------- *)
 (*  Correctness Game (FO Transform)    *)
@@ -116,6 +250,12 @@ proc.
 call eqv_dec; call eqv_enc; call (_ : true); call eqv_kg.
 by auto.
 qed.
+
+lemma eq_Pr_Correctness_Game_Reg_Alt (A <: Adv_Cor) &m :
+  Pr[Correctness_Game(Saber_PKE_Scheme, A).main() @ &m : res]
+  =
+  Pr[Correctness_Game(Saber_PKE_Scheme_Alt, A).main() @ &m : res].
+proof. by byequiv (eqv_Correctness_Game_Reg_Alt A). qed.
 
 (* ----------------------------------- *)
 (*  Correctness Analysis               *)
@@ -160,7 +300,6 @@ op m'_expression_Rq (_A : Rq_mat) (s s': Rq_vec) (m : R2) : Rq =
   let v = v_expression _A s s' in
   let cmq = cmq_expression _A s s' m in
   v - cmq + (upscaleRq h2 (eq - ep)).
-
 op m'_expression (_A : Rq_mat) (s s': Rq_vec) (m : R2) : R2 = 
   scaleRq2R2 (m'_expression_Rq _A s s' m).
 (*
@@ -186,17 +325,28 @@ rewrite /cmq_expression /cmq_expression_centered /v'_expression /error_cmq_cente
 by ring.
 qed.
 
-lemma eq_upscaleRqh2_q4minq4t : upscaleRq h2 (eq - ep) = q4_Rq - q4t_Rq.
+lemma eq_errcmq_errcmqnom (_A : Rq_mat) (s s': Rq_vec) (m : R2) :
+  error_cmq _A s s' m = error_cmq_nom _A s s'.
 proof.
-rewrite /upscaleRq polyXnD1_sumN -(BigRq.XnD1CA.big_split) /=.
-rewrite !(BigRq.XnD1CA.big_seq) &(BigRq.XnD1CA.eq_bigr) /= => i /mem_range rng_i.
-rewrite -scaleN -scaleDl; congr.
-rewrite /h2 rcoeffZ_sum //= /upscaleZq /upscale /shl -inzmodD !inzmodK -eq_inzmod /=.
-rewrite modzMml (pmod_small (2 ^ (eq - et - 2))).
-+ by rewrite /q expr_ge0 //= ltz_weexpn2l //; smt(geet2_ep geep1_eq ge3_eq ge0_et).
-rewrite mulrBl -!exprD_nneg; first 4 smt(ge2_ep geet2_ep geep1_eq ge3_eq ge0_et).
-have ->: ep - 2 + (eq - ep) = eq - 2 by ring.
-by have ->: ep - et - 2 + (eq - ep) = eq - et - 2 by ring.
+rewrite /error_cmq /error_cmq_nom /errorRq /=.
+have ->:
+  scaleR2t2Rq (scaleRq2R2t (v'_expression _A s s' + scaleR22Rq m))
+  =
+  scaleR2t2Rq (scaleRq2R2t (v'_expression _A s s')) + scaleR22Rq m.
++ rewrite -BigRq.XnD1CA.big_split /=.
+  have ->:
+    (fun (i : int) => scaleZ2t2Zq (scaleRq2R2t (v'_expression _A s s')).[i] ** exp Rq.iX i +
+     scaleZ22Zq m.[i] ** exp Rq.iX i)
+    =
+    (fun (i : int) => (scaleZ2t2Zq (scaleRq2R2t (v'_expression _A s s')).[i] + scaleZ22Zq m.[i])  
+     ** exp Rq.iX i).
+  - by rewrite fun_ext /(==) => x; rewrite scaleDl.
+  rewrite polyXnD1_eqP => i rng_i; rewrite !rcoeffZ_sum //= !rcoeffZ_sum //= rcoeffD rcoeffZ_sum //=.
+  rewrite scaleZq2Z2t_DM; first right; rewrite inzmodK /upscale /shl; move: (Z2_asint_values m.[i]). 
+  case => -> /=; first apply dvdz0.
+  - rewrite pmod_small 1:expr_ge0 2:ltz_weexpn2l 7:dvdz_exp2l; smt(ge0_et geet2_ep geep1_eq ge3_eq).
+  by rewrite scaleZ2t2Zq_DM scaleZ22Zq2Z2t2Zq_inv. 
+by ring.
 qed.
 
 lemma eq_expression_m'_m'_alt_Rq (_A : Rq_mat) (s s': Rq_vec) (m : R2) :
@@ -212,6 +362,172 @@ lemma eq_expression_m'_m'_alt (_A : Rq_mat) (s s': Rq_vec) (m : R2) :
    m'_expression _A s s' m = m'_expression_alt _A s s' m.
 proof. by rewrite /m'_expression /m'_expression_alt eq_expression_m'_m'_alt_Rq. qed.
 
+(* --- Delta-Related Errors, Predicates, Properties, and Game --- *)
+(* Error With Probability Distribution That is Computed Exhaustively in Python Script *)
+op delta_error (_A : Rq_mat) (s s' : Rq_vec) = 
+  dotp (error_bq' _A s') s - dotp (error_bq _A s) s' - error_cmq_nom_centered _A s s'.
+
+(* Error Equivalent to Previous Error, But Includes Message m *)
+op delta_error_wm (_A : Rq_mat) (s s' : Rq_vec) (m : R2) = 
+  dotp (error_bq' _A s') s - dotp (error_bq _A s) s' - error_cmq_centered _A s s' m.
+
+(* Predicate That Checks Whether Coefficients are In Correctness Range that Gives Delta Bound *)
+op coeffs_in_correctness_rng (p : Rq) = forall (i : int), 0 <= i < n =>
+  Zq.asint (Zq.inzmod (- q %/ 4)) <= Zq.asint p.[i] \/ Zq.asint p.[i] < Zq.asint (Zq.inzmod (q %/ 4)).
+
+(* Game Used to Represent Delta Bound for the Relevant Error to Have Coefficient in Correct Range *)
+module Delta_Bound_Game = {
+   proc main() : bool = {
+      var sd: seed;
+      var _A : Rq_mat;
+      var s, s': Rq_vec;
+
+      sd <$ dseed;
+      _A <- gen sd;
+      s <$ dsmallRq_vec;
+      s' <$ dsmallRq_vec;
+
+      return coeffs_in_correctness_rng (delta_error _A s s');
+   }
+}.
+
+(* Define Delta Bound and State Delta-Correctness *)
+op delta_bound : real.
+
+axiom delta_correctness &m : 
+  Pr[Delta_Bound_Game.main() @ &m : res] >= 1%r - delta_bound.
+
+(* Equivalence of Delta Errors With and Without m *)
+lemma eq_deltaerror_deltaerrorwm (_A : Rq_mat) (s s' : Rq_vec) (m : R2) :
+   delta_error _A s s' = delta_error_wm _A s s' m.
+proof. 
+by rewrite /delta_error /delta_error_wm /error_cmq_nom_centered /error_cmq_centered 
+           eq_errcmq_errcmqnom.
+qed.
+
+(* --- Proof of Equivalence of Correctness Game for Original Scheme and Delta-Bound Game --- *)
+(* - Intermediate Game, Correctness Game in Terms of Error - *)
+module Correctness_Game_Error (A : Adv_Cor) = {
+   proc main() : bool = {
+      var sd: seed;
+      var _A: Rq_mat;
+      var s, s': Rq_vec;
+      var m: plaintext;
+      
+      sd <$ dseed;
+      _A <- gen sd;
+      s <$ dsmallRq_vec;
+      m <@ A.choose(pk_encode_s (sd, scaleRqv2Rpv (_A *^ s + h)), sk_encode_s s);      
+      s' <$ dsmallRq_vec;
+     
+      return (m_decode m = m'_expression _A s s' (m_decode m));
+   }
+}.
+
+lemma eq_returns_Error_Delta (_A : Rq_mat) (s s' : Rq_vec) (m : R2) :
+  (m = m'_expression _A s s' m) = coeffs_in_correctness_rng (delta_error _A s s').
+proof.
+rewrite /coeffs_in_correctness_rng scaleRq2R2_rng_zero_q4 eq_expression_m'_m'_alt
+        (eq_deltaerror_deltaerrorwm _ _ _ m) /delta_error_wm. 
+rewrite /m'_expression_alt /m'_expression_Rq_alt scaleRq2R2_DM_invl eq_iff.
+split => [eqm_merr | coeffs_corr].
++ by rewrite eq_sym &(addrI m) addr0 {1}eqm_merr; do 2! congr; ring.
++ by rewrite &(addrI (- m)) addrC subrr addrCA addrA subrr add0r -coeffs_corr; congr; ring.
+qed.
+
+lemma eq_Pr_Error_Delta (A <: Adv_Cor) &m:
+  Pr[Correctness_Game_Error(A).main() @ &m : res] 
+  = 
+  Pr[Delta_Bound_Game.main() @ &m : res].
+proof.
+byequiv => //.
+proc.
+wp; rnd; call {1} (_ : true ==> true); auto; first apply (Adv_Cor_ll A).
+progress.
+by rewrite eq_returns_Error_Delta. 
+qed.
+
+lemma eq_Pr_Corr_Error (A <: Adv_Cor) &m:
+  Pr[Correctness_Game(Saber_PKE_Scheme_Alt, A).main() @ &m : res] 
+  = 
+  Pr[Correctness_Game_Error(A).main() @ &m : res].
+proof.
+byequiv => //.
+proc; inline *.
+wp; rnd; wp; call (_ : true); auto.
+progress.
+rewrite !pks_enc_dec_inv !cs_enc_dec_inv !sks_enc_dec_inv /=.
+rewrite /m'_expression /m'_expression_Rq /cmq_expression /v_expression /v'_expression /= eq_sym.
+pose a := dotp (trmx (gen sdL) *^ s'L + error_bq' (gen sdL) s'L) sL.
+have ->: a = dotp (scaleRpv2Rqv (scaleRqv2Rpv (trmx (gen sdL) *^ s'L + h))) sL.
++ rewrite /a /error_bq' /errorRqv; congr. 
+  by rewrite Mat_Rq.Vector.ZModule.addrCA Mat_Rq.Vector.ZModule.addrC Mat_Rq.Vector.ZModule.subrr
+             Mat_Rq.Vector.ZModule.add0r.
+(*
+have ->: b = dotp (scaleRpv2Rqv (scaleRqv2Rpv (gen sdL *^ sL + h))) s'L.
+  - rewrite /b /error_bq /errorRqv; congr.
+    by rewrite Mat_Rq.Vector.ZModule.addrCA Mat_Rq.Vector.ZModule.addrC Mat_Rq.Vector.ZModule.subrr
+               Mat_Rq.Vector.ZModule.add0r.
+*)
+rewrite eq_sym eq_iff; split => [{1}-> | resR_dec].
++ rewrite m_enc_dec_inv eq_sym; do 3! congr. 
+  rewrite /error_cmq /v'_expression /error_bq /errorRqv /errorRq /=; ring.
+  pose b:= gen sdL *^ sL + (scaleRpv2Rqv (scaleRqv2Rpv (gen sdL *^ sL + h)) - gen sdL *^ sL).
+  have ->: b = (scaleRpv2Rqv (scaleRqv2Rpv (gen sdL *^ sL + h))); 2: by ring.
+  - by rewrite /b Mat_Rq.Vector.ZModule.addrCA Mat_Rq.Vector.ZModule.addrC Mat_Rq.Vector.ZModule.subrr
+               Mat_Rq.Vector.ZModule.add0r.
+admit.
+qed.
+
+lemma delta_correctness_original_scheme (A <: Adv_Cor) &m :
+  Pr[Correctness_Game(Saber_PKE_Scheme, A).main() @ &m : res] >= 1%r - delta_bound.
+proof.
+rewrite (eq_Pr_Correctness_Game_Reg_Alt A) (eq_Pr_Corr_Error A) (eq_Pr_Error_Delta  A).
+by apply delta_correctness.
+qed.
+
+(*
+lemma eqv_correrr2_correrrfin (A <: Adv_Cor) &m :
+  Pr[Correctness_Error_Game(A).main() @ &m : res]
+  =
+  Pr[Correctness_Error_Game_Fin.main() @ &m : res].
+proof.
+byequiv => //.
+proc.
+wp. 
+rnd.
+call {1} (_ : true ==> true).
+rnd.
+wp.
+rnd.
+skip.
+progress.
+by rewrite eq_err_errnom_fin.
+qed.
+
+
+(*
+congr. rewrite /error_cmq  /v'_expression /error_bq /errorRqv /errorRq /=. ring. ring. ring.
+  pose a := dotp (trmx (gen sdL) *^ s'L + error_bq' (gen sdL) s'L) sL.
+  have ->: a = dotp (scaleRpv2Rqv (scaleRqv2Rpv (trmx (gen sdL) *^ s'L + h))) sL.
+  - rewrite /a /error_bq' /errorRqv; congr. 
+    by rewrite Mat_Rq.Vector.ZModule.addrCA Mat_Rq.Vector.ZModule.addrC Mat_Rq.Vector.ZModule.subrr
+               Mat_Rq.Vector.ZModule.add0r. 
+  congr; rewrite /error_cmq /v'_expression /errorRq /=; ring.
+  pose b := dotp (gen sdL *^ sL + error_bq (gen sdL) sL) s'L.
+  have ->: b = (dotp (scaleRpv2Rqv (scaleRqv2Rpv (gen sdL *^ sL + h))) s'L); 2: by ring.
+  - rewrite /b /error_bq /errorRqv; congr.
+    by rewrite Mat_Rq.Vector.ZModule.addrCA Mat_Rq.Vector.ZModule.addrC Mat_Rq.Vector.ZModule.subrr
+               Mat_Rq.Vector.ZModule.add0r.
++
+
+pose b := (dotp (gen sdL *^ sL + error_bq (gen sdL) sL) s'L + upscaleRq h1 (eq - ep) +
+          scaleR22Rq (m_decode result_R) + error_cmq (gen sdL) sL s'L (m_decode result_R)).
+ congr. congr.
+rewrite /error_cmq /v'_expression  /error_bq /error_bq' /errorRqv /errorRq /=.
+ ring.
+split => [resR | resR_dec].
+rewrite {1}resR.
 (*
 op m'_expression_reduced_Rq (_A : Rq_mat) (s s': Rq_vec) (m : R2) : Rq =
    scaleR22Rq m + dotp (error_bq' _A s') s - dotp (error_bq _A s) s' 
@@ -335,136 +651,9 @@ module Correctness_Error_Game (S : Scheme, A : Adv_Cor) = {
 *)
 
 
-lemma extract_m_from_m'_Zq (m : Z2) (err : Zq) : 
-  scaleZq2Z2 (scaleZ22Zq m + err) = m + scaleZq2Z2 err.
-proof. 
-rewrite scaleZq2Z2_DM 2:scaleZ22Zq_scaleZq2Z2_inv //; left.
-rewrite /scaleZ22Zq /upscale /shl inzmodK pmod_small 2:dvdz_mull 2:dvdzz.
-move: (Z2_asint_values m); case => -> /= @/q.
-+ by rewrite expr_gt0.
-+ by rewrite expr_ge0 //= ltz_weexpn2l; smt(ge3_eq).
-qed.
 
-lemma scaleZq2Z2_rng_zero (z : Zq) : 
-  Zq.asint Zq.zero <= Zq.asint z < Zq.asint (Zq.inzmod (q %/ 2)) <=> scaleZq2Z2 z = Z2.zero.
-proof.
-rewrite eqv_q2_2eq1 zeroE inzmodK pmod_small 1:expr_ge0 2:ltz_weexpn2l //; 1, 2, 3: smt(ge3_eq). 
-split => [|eq0_scale].
-+ by case => [ge0_z ltq2_z @/scaleZq2Z2 @/downscale @/shr]; rewrite pdiv_small.  
-+ split => [|?].
-  - by rewrite Zq.ge0_asint.
-  - move: eq0_scale; rewrite &(contraLR) ltzNge /=; move: (Zq.gtp_asint z) => @/q ltq_z geq2_z.
-    have ->: (scaleZq2Z2 z <> Z2.zero) = (scaleZq2Z2 z = Z2.one).
-    * move: (Z2_asint_values (scaleZq2Z2 z)); rewrite -zeroE -oneE 2!asint_eq.
-      case => -> /=; rewrite -eq_inzmod //.    
-    rewrite /scaleZq2Z2 /downscale /shr -eq_inzmod; do 2! congr.
-    rewrite eqz_leq -(ler_add2l 1) lez_add1r /= ltz_divLR 2:lez_divRL 1,2:expr_gt0 //=.
-    by rewrite -{1}expr1 -exprD_nneg; 2: smt(ge3_eq).
-qed.
 
-lemma scaleZq2Z2_rng_zero_q4 (err : Zq) :
-  Zq.asint (Zq.inzmod (- q %/ 4)) <= Zq.asint err \/ Zq.asint err < Zq.asint (Zq.inzmod (q %/ 4))
-  <=> 
-  scaleZq2Z2 (Zq.inzmod (q %/ 4) + err) = Z2.zero.
-proof.
-rewrite eq_minq4_q34_modq.
-rewrite -scaleZq2Z2_rng_zero.
-rewrite eqv_q4_2eq2.
-split.
-rewrite zeroE ge0_asint /=.
-case.
-rewrite inzmodK.
-rewrite pmod_small.
-by rewrite mulr_ge0 2:expr_ge0 //= mulrC eq_q_14q_34q eqv_q4_2eq2 mulzC ltz_addr expr_gt0.
-move: (Zq.gtp_asint err) => @/q ltq_err ge34q_err.
-  rewrite eqv_q2_2eq1.
-  rewrite addE !inzmodK modzDml.
-  have tt: exists (x : int), 0 <= x < 2 ^ (eq - 1) /\ 2 ^ (eq - 2) + asint err = q + x.
-  exists (2 ^ (eq - 2) + asint err - q). split. split.
-  - by rewrite -(lez_add2r q) -addzA /= eq_q_14q_34q eqv_q4_2eq2 lez_add2l.
-  - move => ?.
-    rewrite eq_q_14q_34q eqv_q4_2eq2 opprD addzA.
-    smt. smt.
-  move: tt. elim => x. case; case => ge0_x ltq2_x ->.
-  rewrite modzDl !pmod_small 1:ge0_x 2:expr_ge0 //= 1:(ltz_trans (2 ^ (eq - 1))) //
-          /q (_ : 2 ^ eq = 2 ^ (eq - 1) * 2 ^ 1) 1,3: -exprD_nneg //= 2,4:ltr_pmulr 2,5:expr_gt0
-          3,6:expr1; smt(ge3_eq).
 
-rewrite inzmodK pmod_small. smt.
-move: (Zq.ge0_asint err) => ge0_err ltq4_err.
-rewrite addE !inzmodK.
-rewrite (pmod_small (2 ^ (eq - 2))) 1:expr_ge0 //=. smt.
-rewrite !pmod_small. smt. smt.
-rewrite eqv_q2_2eq1 (_ : 2 ^ (eq - 1) = 2 * 2 ^ (eq - 2)) 1:-{2}expr1 1:-exprD_nneg //; 1:smt(ge3_eq).
-rewrite mulrC -intmulz mulr2z ltr_add2l //.
-
-rewrite !addE !inzmodK //= (pmod_small (2 ^ (eq - 2))) 2:(pmod_small (q %/ 2)) 3:(pmod_small (3 * 2 ^ (eq - 2))); 1,2,3: smt.
-rewrite &(contraLR) andaE negb_or negb_and -!ltzNge /= -!lezNgt /=.
-case. move: (Zq.rg_asint err); case => ge0_err ltq_err ltq34_err geq2_err.
-right.
-rewrite pmod_small.
-rewrite addr_ge0 1:expr_ge0 2:ge0_asint //=.
-rewrite eq_q_14q_34q eqv_q4_2eq2 ltr_add2l //.
-rewrite (_ : q %/ 2 = 2 ^ (eq - 2) + 2 ^ (eq - 2)).
-rewrite eqv_q2_2eq1 -mulr2z intmulz -{4}expr1 -exprD_nneg //=; 1: smt(ge3_eq).
-by rewrite lez_add2l.
-qed.
-
-lemma correct_errrng_Zq (m : Z2) (err : Zq) :
-  Zq.asint Zq.zero <= Zq.asint err < Zq.asint (Zq.inzmod (q %/ 2)) 
-  <=> 
-  m = scaleZq2Z2 (scaleZ22Zq m + err).
-proof.
-rewrite extract_m_from_m'_Zq (_ : (m = m + (scaleZq2Z2 err)) <=> ((scaleZq2Z2 err) = Z2.zero)).
-+ split => equ.
-  - by rewrite &(Z2.ZModpRing.addrI m) Z2.ZModpRing.addr0 eq_sym.
-  - by rewrite &(Z2.ZModpRing.addrI (- m)) Z2.ZModpRing.addrA Z2.ZModpRing.addrC Z2.ZModpRing.subrr
-               Z2.ZModpRing.add0r eq_sym.
-+ by apply scaleZq2Z2_rng_zero.
-qed.
-
-lemma extract_m_from_m'_Rq (m : R2) (err : Rq) : 
-  scaleRq2R2 (scaleR22Rq m + err) = m + scaleRq2R2 err.
-proof.
-rewrite polyXnD1_eqP => i rng_i; rewrite rcoeffZ_sum //= 2!rcoeffD. 
-by rewrite rcoeffZ_sum //= rcoeffZ_sum //=  extract_m_from_m'_Zq.
-qed.
-
-lemma scaleRq2R2_rng_zero (p : Rq) : 
-  (forall (i : int), 0 <= i < n => Zq.asint Zq.zero <= Zq.asint p.[i] < Zq.asint (Zq.inzmod (q %/ 2)))
-  <=> 
-  (scaleRq2R2 p = R2.zeroXnD1).
-proof.
-split => [coeff_rng|]; rewrite polyXnD1_eqP => [i rng_i| coeff_scale i rng_i]; 
-         2: move: (coeff_scale i rng_i); rewrite rcoeffZ_sum //= rcoeff0 -scaleZq2Z2_rng_zero //. 
-+ by apply (coeff_rng i rng_i).
-qed.
-
-lemma scaleRq2R2_rng_zero_q4 (err : Rq) :
-  (forall (i : int), 0 <= i < n =>
-   Zq.asint (Zq.inzmod (- q %/ 4)) <= Zq.asint err.[i] 
-   \/ Zq.asint err.[i] < Zq.asint (Zq.inzmod (q %/ 4)))
-  <=> 
-  scaleRq2R2 (q4_Rq + err) = R2.zeroXnD1.
-proof.
-split => [coeff_rng|]; rewrite polyXnD1_eqP => [i rng_i| coeff_scale i rng_i];
-         2: move: (coeff_scale i rng_i); rewrite rcoeffZ_sum //= (Rq.rcoeffD q4_Rq err) rcoeff0
-         rcoeffZ_sum //= -/(Zq.Sub.insubd (2 ^ (eq - 2) %% q)) -/(Zq.inzmod ((2 ^ (eq - 2))))
-         -eqv_q4_2eq2 -(scaleZq2Z2_rng_zero_q4 err.[i]) //.
-+ by apply (coeff_rng i rng_i).
-qed.
-
-lemma correct_errrng_Rq (m : R2) (err : Rq) :
-  (forall (i : int), 0 <= i < n => 
-   Zq.asint Zq.zero <= Zq.asint err.[i] < Zq.asint (Zq.inzmod (q %/ 2)))
-  <=>
-  m = scaleRq2R2 (scaleR22Rq m + err).
-proof.
-split => [coeff_rng|]; rewrite polyXnD1_eqP => [i rng_i| coeff_scale i rng_i];
-         2: move: (coeff_scale i rng_i); rewrite rcoeffZ_sum //= rcoeffD rcoeffZ_sum //=
-         -correct_errrng_Zq //.
-+ by apply (coeff_rng i rng_i).
-qed.
 
 
 (*
@@ -478,11 +667,11 @@ op delta_error (_A : Rq_mat) (s s' : Rq_vec) (m : R2) =
 op delta_error_nom (_A : Rq_mat) (s s' : Rq_vec) = 
   dotp (error_bq' _A s') s - dotp (error_bq _A s) s' - error_cmq_nom_centered _A s s'.
 
-op coefficients_in_delta_rng (p : Rq) = forall (i : int), 0 <= i < n =>
+op coefficients_in_correctness_rng (p : Rq) = forall (i : int), 0 <= i < n =>
   Zq.asint (Zq.inzmod (- q %/ 4)) <= Zq.asint p.[i] \/ Zq.asint p.[i] < Zq.asint (Zq.inzmod (q %/ 4)).
 
 (* Error Game *)
-module Correctness_Error = {
+module Delta_Bound_Game  = {
    proc main(m : R2) : bool = {
       var sd: seed;
       var _A: Rq_mat;
@@ -493,7 +682,7 @@ module Correctness_Error = {
       s <$ dsmallRq_vec;
       s' <$ dsmallRq_vec;
      
-      return coefficients_in_delta_rng (delta_error _A s s' m);
+      return coefficients_in_correctness_rng (delta_error _A s s' m);
    }
 }.
 
@@ -1101,5 +1290,7 @@ m' = m iff 0 <= u' s - u s' - u'' + q/4 < q/2
 m' = m iff - q/4 <= u' s - u s' - u'' < q/4
 
 
+*)
+*)
 *)
 *)
